mem_lessdef results and new mem_lessalloc

veric/mem_lessdef.v
@@ -42,13 +42,86 @@ Definition mem_lessdef m1 m2 :=
   (forall b ofs k p,
       Mem.perm m1 b ofs k p ->
       Mem.perm m2 b ofs k p) /\
-  Mem.nextblock m1 =
-  Mem.nextblock m2.
+  (Mem.nextblock m1 <=
+   Mem.nextblock m2)%positive.
+
+Definition mem_lessalloc m1 m2 :=
+  Mem.loadbytes m1 = Mem.loadbytes m2 /\
+  Mem.perm m1 = Mem.perm m2 /\
+  (Mem.nextblock m1 <= Mem.nextblock m2)%positive.
 
 Definition mem_equiv m1 m2 :=
   Mem.loadbytes m1 = Mem.loadbytes m2 /\
   Mem.perm m1 = Mem.perm m2 /\
   Mem.nextblock m1 = Mem.nextblock m2.
+
+Lemma same_loadbytes_spec m1 m2 :
+  Mem.perm m1 = Mem.perm m2 ->
+  Mem.loadbytes m1 = Mem.loadbytes m2 <->
+  (forall x, Mem.perm_order' (access_at m1 x Cur) Readable -> contents_at m1 x = contents_at m2 x).
+Proof.
+  intros P; split; intros E.
+  - intros (b, ofs) R.
+    Transparent Mem.loadbytes.
+    unfold Mem.loadbytes in *.
+    apply equal_f with (x := b) in E.
+    apply equal_f with (x := ofs) in E.
+    apply equal_f with (x := 1) in E.
+    unfold access_at in *.
+    if_tac [p1|np1] in E; if_tac in E; try discriminate.
+    + simpl in E.
+      unfold contents_at in *.
+      simpl.
+      congruence.
+    + destruct np1.
+      intros ofs1 r1.
+      cut (ofs1 = ofs). intros <-. apply R.
+      omega.
+  - extensionality b ofs k.
+    unfold Mem.loadbytes in *.
+    if_tac [p1|np1]; if_tac [p2|np2].
+    + destruct (zle 0 k).
+      * clear p2.
+        f_equal.
+        rewrite <-(Coqlib.nat_of_Z_eq k) in p1. 2:omega.
+        revert p1. generalize (nat_of_Z k); clear k l; intros n.
+        revert ofs.
+        induction n; auto; intros ofs p.
+        simpl. f_equal.
+        -- spec E (b, ofs).
+           unfold contents_at in *.
+           simpl in E.
+           apply E.
+           apply p.
+           simpl.
+           zify; omega.
+        -- apply IHn.
+           intros ofs' r'.
+           apply p.
+           zify. omega.
+      * rewrite nat_of_Z_neg. auto. omega.
+    + destruct np2.
+      unfold Mem.range_perm in *.
+      rewrite <-P.
+      auto. 
+    + destruct np1.
+      unfold Mem.range_perm in *.
+      rewrite P.
+      auto.
+    + auto.
+Qed.
+
+Definition mem_equiv' m1 m2 :=
+  (forall x, Mem.perm_order' (access_at m1 x Cur) Readable -> contents_at m1 x = contents_at m2 x) /\
+  Mem.perm m1 = Mem.perm m2 /\
+  Mem.nextblock m1 = Mem.nextblock m2.
+
+Lemma mem_equiv'_spec m1 m2 : mem_equiv m1 m2 <-> mem_equiv' m1 m2.
+Proof.
+  split; intros (? & ? & ?); repeat split; auto.
+  rewrite <-same_loadbytes_spec; auto.
+  rewrite same_loadbytes_spec; auto.
+Qed.
 
 Lemma val_inject_antisym v1 v2 :
   val_inject inject_id v1 v2 ->
@@ -87,7 +160,9 @@ Proof.
     apply memval_lessdef_antisym; auto.
   - repeat extensionality.
     apply prop_ext; split; auto.
-  - apply N1.
+  - zify.
+    cut (Z.pos (Mem.nextblock m2) = Z.pos (Mem.nextblock m1)).
+    congruence. omega.
 Qed.
 
 Lemma mem_equiv_refl m : mem_equiv m m.
@@ -95,9 +170,19 @@ Proof.
   split3; hnf; auto.
 Qed.
 
+Lemma mem_lessalloc_refl m : mem_lessalloc m m.
+Proof.
+  split3; auto. apply Ple_refl.
+Qed.
+
 Lemma mem_equiv_refl' m m' : m = m' -> mem_equiv m m'.
 Proof.
   intros <-; apply mem_equiv_refl.
+Qed.
+
+Lemma mem_lessalloc_refl' m m' : m = m' -> mem_lessalloc m m'.
+Proof.
+  intros <-; apply mem_lessalloc_refl.
 Qed.
 
 Lemma mem_equiv_sym m1 m2 : mem_equiv m1 m2 -> mem_equiv m2 m1.
@@ -114,7 +199,23 @@ Proof.
   intros (-> & -> & ->) (-> & -> & ->); auto.
 Qed.
 
-Lemma mem_equiv_lessdef m1 m2 : mem_equiv m1 m2 -> mem_lessdef m1 m2.
+Lemma mem_lessalloc_trans m1 m2 m3 :
+  mem_lessalloc m1 m2 ->
+  mem_lessalloc m2 m3 ->
+  mem_lessalloc m1 m3.
+Proof.
+  unfold mem_lessalloc in *.
+  intros (-> & -> & l) (-> & -> & l'); split; auto. split; auto.
+  eapply Ple_trans; eauto.
+Qed.
+
+Lemma mem_equiv_lessalloc m1 m2 : mem_equiv m1 m2 -> mem_lessalloc m1 m2.
+Proof.
+  intros (L1 & P1 & N1); repeat split; auto.
+  rewrite N1; auto. apply Ple_refl.
+Qed.
+
+Lemma mem_lessalloc_lessdef m1 m2 : mem_lessalloc m1 m2 -> mem_lessdef m1 m2.
 Proof.
   intros (L1 & P1 & N1); repeat split.
   - rewrite L1; auto.
@@ -124,7 +225,13 @@ Proof.
     induction v; constructor; auto.
     apply memval_lessdef_refl.
   - rewrite P1; auto.
-  - rewrite N1; auto.
+  - auto.
+Qed.
+
+Lemma mem_equiv_lessdef m1 m2 : mem_equiv m1 m2 -> mem_lessdef m1 m2.
+Proof.
+  intro H.
+  apply mem_lessalloc_lessdef, mem_equiv_lessalloc, H.
 Qed.
 
 Lemma cl_step_mem_lessdef_sim {ge c m1 c' m1' m2} :
@@ -134,7 +241,19 @@ Lemma cl_step_mem_lessdef_sim {ge c m1 c' m1' m2} :
     mem_lessdef m1' m2' /\
     @cl_step ge c m2 c' m2'.
 Admitted.
- 
+
+Lemma cl_step_mem_lessalloc_sim {ge c m1 c' m1' m2} :
+  mem_lessalloc m1 m2 ->
+  @cl_step ge c m1 c' m1' ->
+  exists m2',
+    mem_lessalloc m1' m2' /\
+    @cl_step ge c m2 c' m2'.
+(* we cannot use [cl_step_mem_lessdef_sim] directly because
+[mem_lessalloc] does not imply [mem_lessdef] in both
+directions. However, the proof must be simpler. *)
+Proof.
+Admitted.
+
 Lemma cl_step_mem_equiv_sim {ge c m1 c' m1' m2} :
   mem_equiv m1 m2 ->
   @cl_step ge c m1 c' m1' ->
@@ -156,6 +275,10 @@ Qed.
 
 Definition juicy_mem_equiv jm1 jm2 := mem_equiv (m_dry jm1) (m_dry jm2) /\ m_phi jm1 = m_phi jm2.
 
+Definition juicy_mem_lessdef jm1 jm2 := mem_lessdef (m_dry jm1) (m_dry jm2) /\ m_phi jm1 = m_phi jm2.
+
+Definition juicy_mem_lessalloc jm1 jm2 := mem_lessdef (m_dry jm1) (m_dry jm2) /\ m_phi jm1 = m_phi jm2.
+
 Lemma mem_equiv_juicy_mem_equiv jm1 m2 :
   mem_equiv (m_dry jm1) m2 ->
   exists jm2,
@@ -169,6 +292,26 @@ Proof.
   all: destruct E as (Load & Perm & Next).
     (* I'll admit this for now. It should take less time to prove once
     the new mem interface is there. *)
+Admitted.
+
+Lemma mem_lessdef_juicy_mem_lessdef jm1 m2 :
+  mem_lessdef (m_dry jm1) m2 ->
+  exists jm2,
+    m_dry jm2 = m2 /\
+    juicy_mem_lessdef jm1 jm2.
+Proof.
+  (* not sure about that one! [contents_cohere] should be ok, but
+  [access_cohere] does not have a reason to be *)
+Admitted.
+
+Lemma mem_lessalloc_juicy_mem_lessdef jm1 m2 :
+  mem_lessalloc (m_dry jm1) m2 ->
+  exists jm2,
+    m_dry jm2 = m2 /\
+    juicy_mem_lessalloc jm1 jm2.
+Proof.
+  (* this one is fine, we need to prove that if two memories are
+  mem_lessalloc then the difference of nextblock is only None's *)
 Admitted.
 
 Lemma juicy_step_mem_equiv_sim {ge c jm1 c' jm1' jm2} :
@@ -188,6 +331,41 @@ Proof.
   - repeat rewrite level_juice_level_phi in *.
     congruence.
 Qed.
+
+Ltac sync D :=
+  first
+    [ split; [destruct D as [D _] | destruct D as [_ D]]
+    | destruct D as [D|D]; [left|right]
+    | let x := fresh in intro x; spec D x
+    ].
+
+Lemma juicy_step_mem_lessdef_sim {ge c jm1 c' jm1' jm2} :
+  juicy_mem_lessdef jm1 jm2 ->
+  corestep (juicy_core_sem cl_core_sem) ge c jm1 c' jm1' ->
+  exists jm2',
+    juicy_mem_lessdef jm1' jm2' /\
+    corestep (juicy_core_sem cl_core_sem) ge c jm2 c' jm2'.
+Proof.
+  intros [Ed Ew] [step D].
+  destruct (cl_step_mem_lessdef_sim Ed step) as [m2' [Ed' Sd']].
+  destruct (mem_lessdef_juicy_mem_lessdef jm1' m2' Ed') as (jm2', (<-, [Hd Hw])).
+  exists jm2'.
+  split; split; auto.
+  repeat rewrite level_juice_level_phi in *.
+  
+  repeat sync D.
+  
+  all: try rewrite <-Ew; try rewrite <-Hw; try assumption.
+  
+  - intros out. apply D.
+    unfold mem_lessdef in *.
+    zify.
+    omega.
+  
+  - unfold mem_lessdef in *.
+    zify.
+    Fail omega. (* not true, maybe we can still resource_decay them somehow *)
+Admitted.
 
 Definition ext_spec_stable {M E Z} (R : M -> M -> Prop)
            (spec : external_specification M E Z) :=
@@ -225,6 +403,44 @@ Proof.
     destruct (Post ret jm2' z' _ Hargsty Hretty Hn) as (c' & atex' & safe'); auto.
     + split; auto.
       destruct E as [Ed Ew].
+      unfold juicy_safety.pures_eq in *.
+      unfold juicy_safety.pures_sub in *.
+      split.
+      * repeat rewrite level_juice_level_phi in *.
+        congruence.
+      * revert pure.
+        rewrite Ew.
+        auto.
+    + exists c'; split; auto.
+  
+  - econstructor 4; eauto.
+Qed.
+
+Lemma jsafeN_mem_lessdef {Z Jspec ge n z c jm1 jm2} :
+  juicy_mem_lessdef jm1 jm2 ->
+  ext_spec_stable juicy_mem_lessdef (JE_spec _ Jspec) ->
+  @jsafeN Z Jspec ge n z c jm1 ->
+  @jsafeN Z Jspec ge n z c jm2.
+Proof.
+  intros L [Spre Sexit] S1.
+  revert jm2 L.
+  induction S1 as
+      [ z c jm1
+      | n z c jm1 c' jm1' step safe IH
+      | n z c jm1 ef args x atex Pre Post
+      | n z c jm1 v Halt Exit ]; intros jm2 L.
+  
+  - constructor 1.
+  
+  - destruct (juicy_step_mem_lessdef_sim L step) as (jm2' & E' & step').
+    econstructor 2; eauto.
+    apply IH, E'.
+  
+  - econstructor 3 with (x := x); eauto.
+    intros ret jm2' z' n' Hargsty Hretty Hn [-> [lev pure]] post.
+    destruct (Post ret jm2' z' _ Hargsty Hretty Hn) as (c' & atex' & safe'); auto.
+    + split; auto.
+      destruct L as [Ed Ew].
       unfold juicy_safety.pures_eq in *.
       unfold juicy_safety.pures_sub in *.
       split.
